14MachineCode/MachineCode.thy
@@ -2,22 +2,20 @@ theory MachineCode
   imports Main
 begin
 
-datatype register = R1 | R2 | R3 | R4 | R5 | R6
+datatype reg = R1 | R2 | R3 | R4 | R5 | R6
 
 datatype mach = 
-    LDI register nat      (* $R := k *)
-  | LOD register register (* $R\<^sub>1 := M[$R\<^sub>2] *)
-  | STO register register (* M[$R\<^sub>1] := $R\<^sub>2 *)
-  | MOV register register (* $R\<^sub>1 := $R\<^sub>2 *)
-  | ADD register nat      (* $R := $R + k *)
-  | SUB register nat      (* $R := $R - k *)
-  | IJP register          (* $PC := $R (indirect jump) *)
-  | JIZ register nat      (* $R = 0 \<longrightarrow> $PC = $PC + k, $R \<noteq> 0 \<longrightarrow> NOOP (conditional forward jump) *)
-  | JMP nat               (* $PC := $PC - k (backwards jump) *)
+  LDI reg nat (* $R := k *)
+  | LOD reg reg (* $R\<^sub>1 := M[$R\<^sub>2] *)
+  | STO reg reg (* M[$R\<^sub>1] := $R\<^sub>2 *)
+  | STI reg nat (* M[$R] := k *)
+  | MOV reg reg (* $R\<^sub>1 := $R\<^sub>2 *)
+  | MVP reg     (* $R := $PC *)
+  | ADD reg nat (* $R := $R + k *)
+  | SUB reg nat (* $R := $R - k *)
+  | JMP reg     (* $PC := $R (indirect jump) *)
 
-  | ASSERT register "nat \<Rightarrow> bool" (* P($R) \<longrightarrow> NOOP, \<not>P($R) \<longrightarrow> abort *)
-
-datatype mach_state = MS "register \<Rightarrow> nat" "nat \<Rightarrow> nat" nat
+datatype mach_state = MS "reg \<Rightarrow> nat" "nat \<Rightarrow> nat" nat
 
 inductive evalm :: "mach list \<Rightarrow> mach_state \<Rightarrow> mach_state \<Rightarrow> bool" (infix "\<tturnstile> _ \<leadsto>\<^sub>m" 50) where 
   evm_ldi [simp]: "cd ! pc = LDI r k \<Longrightarrow> 
@@ -26,22 +24,18 @@ inductive evalm :: "mach list \<Rightarrow> mach_state \<Rightarrow> mach_state 
     cd \<tturnstile> MS rs mem (Suc pc) \<leadsto>\<^sub>m MS (rs(r := mem (rs ptr))) mem pc"
 | evm_sto [simp]: "cd ! pc = STO ptr r \<Longrightarrow> 
     cd \<tturnstile> MS rs mem (Suc pc) \<leadsto>\<^sub>m MS rs (mem(rs ptr := rs r)) pc"
+| evm_sti [simp]: "cd ! pc = STI ptr k \<Longrightarrow> 
+    cd \<tturnstile> MS rs mem (Suc pc) \<leadsto>\<^sub>m MS rs (mem(rs ptr := k)) pc"
 | evm_mov [simp]: "cd ! pc = MOV r1 r2 \<Longrightarrow> 
     cd \<tturnstile> MS rs mem (Suc pc) \<leadsto>\<^sub>m MS (rs(r1 := rs r2)) mem pc"
+| evm_mvp [simp]: "cd ! pc = MVP r \<Longrightarrow> 
+    cd \<tturnstile> MS rs mem (Suc pc) \<leadsto>\<^sub>m MS (rs(r := pc)) mem pc"
 | evm_add [simp]: "cd ! pc = ADD r k \<Longrightarrow> 
     cd \<tturnstile> MS rs mem (Suc pc) \<leadsto>\<^sub>m MS (rs(r := rs r + k)) mem pc"
 | evm_sub [simp]: "cd ! pc = SUB r k \<Longrightarrow> 
     cd \<tturnstile> MS rs mem (Suc pc) \<leadsto>\<^sub>m MS (rs(r := rs r - k)) mem pc"
-| evm_ijp [simp]: "cd ! pc = IJP r \<Longrightarrow> 
+| evm_jmp [simp]: "cd ! pc = JMP r \<Longrightarrow> 
     cd \<tturnstile> MS rs mem (Suc pc) \<leadsto>\<^sub>m MS rs mem (rs r)"
-| evm_jiz_z [simp]: "cd ! pc = JIZ r k \<Longrightarrow> rs r = 0 \<Longrightarrow>
-    cd \<tturnstile> MS rs mem (Suc pc) \<leadsto>\<^sub>m MS rs mem (pc - k)"
-| evm_jiz_s [simp]: "cd ! pc = JIZ r pc' \<Longrightarrow> rs r = Suc y \<Longrightarrow>
-    cd \<tturnstile> MS rs mem (Suc pc) \<leadsto>\<^sub>m MS rs mem pc"
-| evm_jmp [simp]: "cd ! pc = JMP k \<Longrightarrow> 
-    cd \<tturnstile> MS rs mem (Suc pc) \<leadsto>\<^sub>m MS rs mem (pc + k)"
-| evm_assert [simp]: "cd ! pc = ASSERT r p \<Longrightarrow> p (rs r) \<Longrightarrow> 
-    cd \<tturnstile> MS rs mem (Suc pc) \<leadsto>\<^sub>m MS rs mem pc"
 
 theorem determinismm: "cd \<tturnstile> \<Sigma> \<leadsto>\<^sub>m \<Sigma>' \<Longrightarrow> cd \<tturnstile> \<Sigma> \<leadsto>\<^sub>m \<Sigma>'' \<Longrightarrow> \<Sigma>' = \<Sigma>''"
 proof (induction cd \<Sigma> \<Sigma>' rule: evalm.induct)
@@ -57,8 +51,16 @@ next
   from evm_sto(2, 1) show ?case 
     by (induction cd "MS rs mem (Suc pc)" \<Sigma>'' rule: evalm.induct) simp_all
 next
+  case (evm_sti cd pc ptr k rs mem)
+  from evm_sti(2, 1) show ?case 
+    by (induction cd "MS rs mem (Suc pc)" \<Sigma>'' rule: evalm.induct) simp_all
+next
   case (evm_mov cd pc r1 r2 rs mem)
   from evm_mov(2, 1) show ?case 
+    by (induction cd "MS rs mem (Suc pc)" \<Sigma>'' rule: evalm.induct) simp_all
+next
+  case (evm_mvp cd pc r rs mem)
+  from evm_mvp(2, 1) show ?case 
     by (induction cd "MS rs mem (Suc pc)" \<Sigma>'' rule: evalm.induct) simp_all
 next
   case (evm_add cd pc r k rs mem)
@@ -69,24 +71,8 @@ next
   from evm_sub(2, 1) show ?case 
     by (induction cd "MS rs mem (Suc pc)" \<Sigma>'' rule: evalm.induct) simp_all
 next
-  case (evm_ijp cd pc r rs mem)
-  from evm_ijp(2, 1) show ?case 
-    by (induction cd "MS rs mem (Suc pc)" \<Sigma>'' rule: evalm.induct) simp_all
-next
-  case (evm_jiz_z cd pc r pc' rs mem)
-  from evm_jiz_z(3, 1, 2) show ?case 
-    by (induction cd "MS rs mem (Suc pc)" \<Sigma>'' rule: evalm.induct) simp_all
-next
-  case (evm_jiz_s cd pc r pc' rs y mem)
-  from evm_jiz_s(3, 1, 2) show ?case 
-    by (induction cd "MS rs mem (Suc pc)" \<Sigma>'' rule: evalm.induct) simp_all
-next
-  case (evm_jmp cd pc k rs mem)
+  case (evm_jmp cd pc r rs mem)
   from evm_jmp(2, 1) show ?case 
-    by (induction cd "MS rs mem (Suc pc)" \<Sigma>'' rule: evalm.induct) simp_all
-next
-  case (evm_assert cd pc r p rs mem)
-  from evm_assert(3, 1, 2) show ?case 
     by (induction cd "MS rs mem (Suc pc)" \<Sigma>'' rule: evalm.induct) simp_all
 qed
 
