Correctness.thy
@@ -15,7 +15,7 @@ qed
 theorem tc_terminationn: "compile e = Some cd \<Longrightarrow> 
   \<exists>v. valn v \<and> e \<Down> v \<and> (\<exists>rs mem. rs R3 = 1 \<and> rs R4 = 0 \<and> 
     print_mval mem (4 * mem 2) = print_nexpr v \<and> 
-      iter (\<tturnstile> cd \<leadsto>\<^sub>m) (MS ((\<lambda>r. 0)(R4 := 1)) (nmem(3 := 0)) (length cd)) (MS rs mem 0))"
+      iter (\<tturnstile> cd \<leadsto>\<^sub>m) (MS ((\<lambda>r. 0)(R4 := 2)) (nmem(3 := 0, 7 := 0)) (length cd)) (MS rs mem 0))"
 proof -
   assume C: "compile e = Some cd"
   then obtain e\<^sub>t t where T: "typecheck e = Some (e\<^sub>t, t)" by fastforce
@@ -84,26 +84,27 @@ proof -
     (US h\<^sub>u hp\<^sub>u e\<^sub>u ep\<^sub>u vs\<^sub>u 1 sh\<^sub>u 0 0)" by simp
   hence EU: "iter (\<tturnstile> ?cd \<leadsto>\<^sub>u) (US nmem 0 nmem 0 nmem 0 (nmem(0 := 0, 1 := 0)) 2 (length ?cd)) 
     (US h\<^sub>u hp\<^sub>u e\<^sub>u ep\<^sub>u vs\<^sub>u 1 sh\<^sub>u 0 0)" by simp
-  let ?mem = "(\<lambda>m. case m of Hp \<Rightarrow> h\<^sub>u | Env \<Rightarrow> e\<^sub>u | Val \<Rightarrow> vs\<^sub>u | Stk \<Rightarrow> sh\<^sub>u)"
-  let ?rs = "(\<lambda>r. case r of HP \<Rightarrow> hp\<^sub>u | EP \<Rightarrow> ep\<^sub>u | VP \<Rightarrow> Suc 0 | SP \<Rightarrow> 0 | ACC \<Rightarrow> 0 | AC2 \<Rightarrow> 0)"
-  let ?cd' = "(fst \<circ> assemble) ?cd"
-
-
-
-
-  from C T obtain mp where MP: "assemble ?cd = (?cd', mp)" by (cases "assemble ?cd") simp_all
-  with EU have "iter (\<tturnstile> ?cd' \<leadsto>\<^sub>a) 
-    (assemble_state mp (US nmem 0 nmem 0 nmem 0 (nmem(0 := 0, 1 := 0)) 2 (length ?cd))) 
-      (assemble_state mp (US h\<^sub>u hp\<^sub>u e\<^sub>u ep\<^sub>u vs\<^sub>u 1 sh\<^sub>u 0 0))" by (metis correcta_iter)
-  with MP have "iter (\<tturnstile> ?cd' \<leadsto>\<^sub>a) 
-    (AS (\<lambda>r. if r = SP then 2 else 0) (\<lambda>m. if m = Stk then nmem(0 := 0, 1 := 0) else nmem) 
-      (length ?cd')) (AS ?rs ?mem 0)" by simp 
+  let ?cd' = "assemble_code ?cd"
+  let ?mp = "assembly_map ?cd"
+  let ?mem = "case_register (assm_hp ?cd h\<^sub>u) e\<^sub>u vs\<^sub>u (assm_stk ?cd sh\<^sub>u) nmem nmem"
+  let ?rs = "case_register hp\<^sub>u ep\<^sub>u (Suc 0) 0 0 0"
+  from R EU have "iter (\<tturnstile> ?cd' \<leadsto>\<^sub>a) 
+    (assemble_state ?mp (US nmem 0 nmem 0 nmem 0 (nmem(0 := 0, 1 := 0)) 2 (length ?cd))) 
+      (assemble_state ?mp (US h\<^sub>u hp\<^sub>u e\<^sub>u ep\<^sub>u vs\<^sub>u 1 sh\<^sub>u 0 0))" by (metis correcta_iter)
+  hence "iter (\<tturnstile> ?cd' \<leadsto>\<^sub>a) 
+    (AS (case_register (assm_hp ?cd nmem) nmem nmem ((assm_stk ?cd nmem)(0 := 0, 1 := 0)) nmem nmem) 
+      (case_register 0 0 0 2 0 0) (length ?cd')) (AS ?mem ?rs 0)" by simp 
   hence "iter (\<tturnstile> disassemble ?cd' \<leadsto>\<^sub>m) 
-    (disassemble_state (AS (\<lambda>r. if r = SP then 2 else 0) 
-      (\<lambda>m. if m = Stk then nmem(0 := 0, 1 := 0) else nmem) (length ?cd'))) 
-        (disassemble_state (AS ?rs ?mem 0))" by (metis correctm_iter)
-  with C T have EM: "iter (\<tturnstile> cd \<leadsto>\<^sub>m) (MS ((\<lambda>r. 0)(R4 := 2)) (nmem(3 := 0)) (length cd)) 
-    (MS (?rs \<circ> inv_register_map) (uncurry ?mem \<circ> unmap_mem) 0)" by auto
+    (disassemble_state (AS (case_register (assm_hp ?cd nmem) nmem nmem 
+      ((assm_stk ?cd nmem)(0 := 0, 1 := 0)) nmem nmem) (case_register 0 0 0 2 0 0) (length ?cd')))
+        (disassemble_state (AS ?mem ?rs 0))" by (metis correctm_iter)
+  hence "iter (\<tturnstile> disassemble ?cd' \<leadsto>\<^sub>m) (MS (case_reg 0 0 0 2 0 0)
+    (uncurry (case_register (assm_hp ?cd nmem) nmem nmem ((assm_stk ?cd nmem)(0 := 0, Suc 0 := 0)) 
+      nmem nmem) \<circ> unmap_mem) (list_sum (map assemble_op_len ?cd)))
+        (MS (case_reg hp\<^sub>u ep\<^sub>u (Suc 0) 0 0 0) (uncurry ?mem \<circ> unmap_mem) 0)" 
+    by simp
+  with C T have EM: "iter (\<tturnstile> cd \<leadsto>\<^sub>m) (MS ((\<lambda>r. 0)(R4 := 2)) (nmem(3 := 0, 7 := 0)) (length cd)) 
+    (MS (case_reg hp\<^sub>u ep\<^sub>u (Suc 0) 0 0 0) (uncurry ?mem \<circ> unmap_mem) 0)" by auto
   from EC VT have "print_closure c = print_nexpr (erase v\<^sub>t)" by simp
   moreover from EB have "print_bclosure v\<^sub>b = print_tco_closure (tco_val (encode_closure c))" by simp
   ultimately have "print_bclosure v\<^sub>b = print_nexpr (erase v\<^sub>t)" by simp
@@ -112,13 +113,15 @@ proof -
   with VH have "print_ceclosure (get_closure (flatten_values h\<^sub>c\<^sub>e) (3 * v\<^sub>h)) = print_nexpr (erase v\<^sub>t)" 
     by (simp del: get_closure.simps)
   with VU VSU have "print_uval h\<^sub>u (vs\<^sub>u 0) = print_nexpr (erase v\<^sub>t)" by (metis print_u)
-  hence PU: "print_uval (?mem Hp) (?mem Val 0) = print_nexpr (erase v\<^sub>t)" by simp
-  have "unmap_mem (4 * ?mem Val 0) = (Hp, ?mem Val 0)" by simp
-  hence "unmap_mem (4 * (uncurry ?mem \<circ> unmap_mem) 2) = (Hp, ?mem Val 0)" by (simp add: numeral_def)
-  with PU have PM: "print_mval (uncurry ?mem \<circ> unmap_mem) (4 * (uncurry ?mem \<circ> unmap_mem) 2) = 
-    print_nexpr (erase v\<^sub>t)" by (metis print_m)
-  have "(?rs \<circ> inv_register_map) R3 = 1 \<and> (?rs \<circ> inv_register_map) R4 = 0" by simp
-  with VN TN EN EM PM show ?thesis by blastx
+  with VSU have PA: "print_uval (?mem Hp) (?mem Vals 0) = print_nexpr (erase v\<^sub>t)" 
+    using print_a by simp
+  have "unmap_mem (4 * ?mem Vals 0) = (Hp, ?mem Vals 0)" by simp
+  hence "unmap_mem (4 * (uncurry ?mem \<circ> unmap_mem) 2) = (Hp, ?mem Vals 0)" 
+    by (simp add: numeral_def)
+  with PA have PM: "print_mval (uncurry ?mem \<circ> unmap_mem) (4 * (uncurry ?mem \<circ> unmap_mem) 2) = 
+    print_nexpr (erase v\<^sub>t)" using print_m by presburger
+  have "(case_reg hp\<^sub>u ep\<^sub>u (Suc 0) 0 0 0) R3 = 1 \<and> (case_reg hp\<^sub>u ep\<^sub>u (Suc 0) 0 0 0) R4 = 0" by simp
+  with VN TN EN EM PM show ?thesis by blast
 qed
 
 end
